instantiate and simplify.

theories/STac/Simplify.v
@@ -15,6 +15,14 @@ Section parameterized.
     fun tus tvs s hs e =>
       More nil nil s hs (f tus tvs s e).
 
+(*
+  Definition SIMPLIFY_hyps
+             (f : list typ -> list typ -> subst -> expr -> expr)
+  : stac typ expr subst :=
+    fun tus tvs s hs e =>
+      More nil nil s (List.map (f tus tvs s) hs) e.
+*)
+
   Variable RType_typ : RType typ.
   Variable Expr_expr : Expr RType_typ expr.
   Variable ExprOk_expr : ExprOk Expr_expr.
@@ -37,7 +45,7 @@ Section parameterized.
            | Some eD , Some sD , Some eD' =>
              forall us vs,
                sD us vs ->
-               eD us vs <-> eD' us vs
+               (eD us vs <-> eD' us vs)
          end) ->
       stac_sound (SIMPLIFY f).
   Proof.
@@ -75,5 +83,82 @@ Section parameterized.
       destruct (eq_sym (HList.app_nil_r_trans tvs)).
       rewrite H1. congruence. }
   Qed.
+
+(*
+  Theorem SIMPLIFY_hyps_sound
+  : forall f,
+      (forall tus tvs s e e',
+         WellFormed_subst s ->
+         f tus tvs s e = e' ->
+         match @propD _ _ _ Expr_expr _ tus tvs e
+             , @substD _ _ _ _ Expr_expr _ _ tus tvs s
+             , @propD _ _ _ _ _ tus tvs e'
+         with
+           | None , _ , _ => True
+           | _ , None , _ => True
+           | Some _ , Some _ , None => False
+           | Some eD , Some sD , Some eD' =>
+             forall us vs,
+               sD us vs ->
+               (eD us vs <-> eD' us vs)
+         end) ->
+      stac_sound (SIMPLIFY_hyps f).
+  Proof.
+    intros. unfold stac_sound, SIMPLIFY_hyps.
+    intros.
+    specialize (fun g => H tus tvs s g _ H0 eq_refl).
+    forward.
+    split; auto. clear H0.
+    unfold stateD in *.
+    forward.
+    rewrite propD_conv
+       with (pfu := eq_sym (HList.app_nil_r_trans _))
+            (pfv := eq_sym (HList.app_nil_r_trans _)).
+    rewrite substD_conv
+       with (pfu := eq_sym (HList.app_nil_r_trans _))
+            (pfv := eq_sym (HList.app_nil_r_trans _)).
+    autorewrite with eq_rw.
+    rewrite H0.
+    Opaque Traversable.mapT.
+    rewrite ListMapT.mapT_map.
+    match goal with
+      | |- match match ?X with _ => _ end with _ => _ end =>
+        assert (exists y,
+                  X = Some y /\
+                  forall (us : HList.hlist (typD nil) tus)
+                         (vs : HList.hlist (typD nil) tvs),
+                    P1 us vs ->
+                    Forall2 (fun l r => l us vs <-> r us vs) l y)
+    end.
+
+    match goal with
+      | |- match ?X with _ => _ end =>
+        consider X; intros
+    end.
+    rewrite
+    { forward_reason.
+      forward. inv_all; subst.
+      rewrite (HList.hlist_eta x) in *.
+      rewrite (HList.hlist_eta x0) in *.
+      do 2 rewrite HList.hlist_app_nil_r in H6.
+      destruct (eq_sym (HList.app_nil_r_trans tus)).
+      destruct (eq_sym (HList.app_nil_r_trans tvs)).
+      rewrite H2 in *. rewrite H8 in *. rewrite H7 in *.
+      inv_all; subst.
+      intuition. apply H4; auto. }
+    { revert H5.
+      rewrite propD_conv
+         with (pfu := eq_sym (HList.app_nil_r_trans tus))
+              (pfv := eq_sym (HList.app_nil_r_trans tvs)).
+      rewrite substD_conv
+         with (pfu := eq_sym (HList.app_nil_r_trans tus))
+              (pfv := eq_sym (HList.app_nil_r_trans tvs)).
+      autorewrite with eq_rw.
+      Cases.rewrite_all_goal.
+      destruct (eq_sym (HList.app_nil_r_trans tus)).
+      destruct (eq_sym (HList.app_nil_r_trans tvs)).
+      rewrite H1. congruence. }
+  Qed.
+*)
 
 End parameterized.
