theories/STac/Instantiate.v
@@ -8,11 +8,9 @@ Require Import MirrorCore.Util.ListMapT.
 Require Import MirrorCore.EnvI.
 Require Import MirrorCore.SymI.
 Require Import MirrorCore.SubstI.
-Require Import MirrorCore.Lemma.
-Require Import MirrorCore.LemmaApply.
 Require Import MirrorCore.InstantiateI.
 Require Import MirrorCore.STac.Core.
-Require Import MirrorCore.STac.Continuation.
+Require Import MirrorCore.STac.Simplify.
 
 Set Implicit Arguments.
 Set Strict Implicit.
@@ -25,25 +23,16 @@ Section parameterized.
   Variable Typ0_Prop : Typ0 _ Prop.
   Let tyProp : typ := @typ0 _ _ _ _.
 
-  Variable vars_to_uvars : nat -> nat -> expr -> expr.
-  Variable exprUnify : tenv typ -> tenv typ -> nat -> expr -> expr -> typ -> subst -> option subst.
   Variable instantiate : (nat -> option expr) -> nat -> expr -> expr.
 
   Section instantiate.
     Variable Subst_subst : Subst subst expr.
     Variable SU : SubstUpdate subst expr.
 
-    (** Think of this like:
-     **   apply lem ; cont
-     ** i.e. first apply the lemma and then require that all side-conditions
-     ** except the last are solved by the prover [tac], currently with
-     ** empty facts.
-     **)
     Definition INSTANTIATE
     : stac typ expr subst :=
-      fun tus tvs sub hs e =>
-        let inst := instantiate (fun u => lookup u sub) 0 in
-        More nil nil sub (List.map inst hs) (inst e).
+      @SIMPLIFY typ expr subst
+                (fun tus tvs sub => instantiate (fun u => lookup u sub) 0).
   End instantiate.
 
   Variable Expr_expr : Expr RType_typ expr.
@@ -56,34 +45,21 @@ Section parameterized.
   Theorem INSTANTIATE_sound
   : stac_sound (INSTANTIATE _).
   Proof.
-    intros. red; simpl.
-    intuition.
+    eapply SIMPLIFY_sound.
+    intros. unfold propD.
     forward.
-    unfold stateD in *.
-    Require Import MirrorCore.Util.Forwardy.
-    forwardy.
+    eapply sem_preserves_if_substD in H3; eauto.
+    red in exprD'_instantiate.
+    eapply exprD'_instantiate with (tvs' := nil) in H1; eauto.
+    simpl in H1.
+    forward_reason.
+    subst. rewrite H1.
+    intros.
     inv_all; subst.
-    erewrite substD_conv
-        with (pfu := app_nil_r_trans _) (pfv := app_nil_r_trans _) in H2.
-    unfold ResType in H2.
-    autorewrite with eq_rw in H2.
-    forwardy. inv_all; subst.
-    eapply sem_preserves_if_substD in H2; eauto.
-    specialize (fun g gD =>
-                  @exprD'_instantiate (tus ++ nil) (tvs ++ nil)
-                                      (fun u : nat => lookup u s) g nil tyProp gD _ H2).
-    Opaque mapT.
-    unfold propD in *.
-    forwardy; inv_all; subst.
-    rewrite exprD'_conv
-       with (pfu := app_nil_r_trans _) (pfv := app_nil_r_trans _) in H0.
-    unfold ResType in H0; autorewrite with eq_rw in H0.
-    forwardy.
-    eapply exprD'_instantiate in H0.
-    simpl in *; forward_reason.
-    change_rewrite H0.
-    inv_all; subst.
-    admit.
+    autorewrite with eq_rw.
+    specialize (H4 us vs Hnil).
+    simpl in *.
+    rewrite H4; auto. reflexivity.
   Qed.
 
 End parameterized.
